State rmw to llsc

src/promising/RMWtoLLSC.v
@@ -1,5 +1,4 @@
-From Paco Require Import paco.
-
+Require Import FunctionalExtensionality.
 Require Import Relations.
 Require Import EquivDec.
 Require Import Equality.
@@ -12,7 +11,9 @@ Require Import ZArith.
 Require Import FMapPositive.
 Require Import FSetPositive.
 Require Import EquivDec.
-Require Import sflib.
+
+From sflib Require Import sflib.
+From Paco Require Import paco.
 
 Require Import PromisingArch.lib.Basic.
 Require Import PromisingArch.lib.Order.
@@ -20,8 +21,10 @@ Require Import PromisingArch.lib.Time.
 Require Import PromisingArch.lib.Lang.
 
 Require Import PromisingArch.promising.Promising.
+Require Import PromisingArch.promising.Sim.
 
 Set Implicit Arguments.
+Set Nested Proofs Allowed.
 
 
 Fixpoint rmw_to_llsc_stmt (tmp: Id.t) (stmt: stmtT): list stmtT :=
@@ -41,12 +44,21 @@ Fixpoint rmw_to_llsc_stmt (tmp: Id.t) (stmt: stmtT): list stmtT :=
   | _ => [stmt]
   end.
 
+Definition rmw_to_llsc_stmts (tmp: Id.t) (stmts: list stmtT): list stmtT :=
+  List.fold_right (@List.app _) [] (List.map (rmw_to_llsc_stmt tmp) stmts).
+
+Definition rmw_to_llsc_program (p_src p_tgt: program): Prop :=
+  forall tid, exists tmp,
+    option_rel
+      (fun stmts_src stmts_tgt => stmts_tgt = rmw_to_llsc_stmts tmp stmts_src)
+      (IdMap.find tid p_src) (IdMap.find tid p_tgt).
+
 Inductive fresh (r: Id.t): forall (stmt: stmtT), Prop :=
 | fresh_instr
     i
     (FRESH: ~ IdSet.mem r (regs_of_instr i)):
   fresh r (stmt_instr i)
-| fresh_cond
+| fresh_if
     cond s1 s2
     (FRESH_COND: ~ IdSet.mem r (regs_of_expr cond))
     (FRESH_STMT1: List.Forall (fresh r) s1)
@@ -59,19 +71,221 @@ Inductive fresh (r: Id.t): forall (stmt: stmtT), Prop :=
   fresh r (stmt_dowhile s cond)
 .
 
+Definition is_exclusive (i: instrT): bool :=
+  match i with
+  | instr_load ex _ _ _
+  | instr_store ex _ _ _ _ => ex
+  | _ => false
+  end.
 
-Section SIM.
-  Variant _sim_machine (sim: Machine.t -> Machine.t -> Prop) (m_src m_tgt: Machine.t): Prop :=
-    | _sim_machine_intro:
-      _sim_machine sim m_src m_tgt
-  .
-  #[local] Hint Constructors _sim_machine: paco.
+Inductive exclusive_free: forall (stmt: stmtT), Prop :=
+| exclusive_free_instr
+    i
+    (EXFREE: ~ is_exclusive i):
+  exclusive_free (stmt_instr i)
+| exclusive_free_if
+    cond s1 s2
+    (EXFREE1: List.Forall exclusive_free s1)
+    (EXFREE2: List.Forall exclusive_free s2):
+  exclusive_free (stmt_if cond s1 s2)
+| exclusive_free_dowhile
+    s cond
+    (EXFREE: List.Forall exclusive_free s):
+  exclusive_free (stmt_dowhile s cond)
+.
 
-  Lemma sim_machine_monotone: monotone2 _sim_machine.
+
+Variant sim_val (v_src v_tgt: ValA.t (A:=View.t (A:=unit))): Prop :=
+| sim_val_intro
+    (VAL: ValA.val v_src = ValA.val v_tgt)
+    (ANNOT: le (ValA.annot v_src) (ValA.annot v_tgt))
+.
+
+Definition sim_rmap (tmp: Id.t) (rmap_src rmap_tgt: RMap.t (A:=View.t (A:=unit))): Prop :=
+  forall r (NEQ: r <> tmp),
+    sim_val (RMap.find r rmap_src) (RMap.find r rmap_tgt).
+
+Variant sim_local (lc_src lc_tgt: Local.t (A:=unit)): Prop :=
+| sim_local_intro
+    (COH: lc_src.(Local.coh) = lc_tgt.(Local.coh))
+    (VRN: lc_src.(Local.vrn) = lc_tgt.(Local.vrn))
+    (VWN: lc_src.(Local.vwn) = lc_tgt.(Local.vwn))
+    (VRO: lc_src.(Local.vro) = lc_tgt.(Local.vro))
+    (VWO: lc_src.(Local.vwo) = lc_tgt.(Local.vwo))
+    (VCAP: lc_src.(Local.vcap) = lc_tgt.(Local.vcap))
+    (VREL: lc_src.(Local.vrel) = lc_tgt.(Local.vrel))
+    (FWDBANK: lc_src.(Local.fwdbank) = lc_tgt.(Local.fwdbank))
+    (EXBANK: lc_src.(Local.exbank) = None)
+    (PROMISES: Local.promises lc_src = Local.promises lc_tgt)
+.
+#[export] Hint Constructors sim_local: core.
+
+Lemma sim_local_step
+      e tid mem_tgt lc1_tgt lc2_tgt
+      mem_src lc1_src
+      (LOCAL: sim_local lc1_src lc1_tgt)
+      (MEMORY: mem_src = mem_tgt)
+      (STEP_TGT: Local.step e tid mem_tgt lc1_tgt lc2_tgt)
+      (EXFREE: match e with
+               | Event.read ex _ _ _
+               | Event.write ex _ _ _ _ => ex = false
+               | _ => True
+               end):
+  exists lc2_src,
+    (<<STEP_SRC: Local.step e tid mem_src lc1_src lc2_src>>) /\
+    (<<LOCAL2: sim_local lc2_src lc2_tgt>>).
+Proof.
+  destruct lc1_src, lc1_tgt. inv LOCAL; ss. subst.
+  inv STEP_TGT; subst.
+  { (* internal *)
+    esplits; [econs 1|]; eauto.
+  }
+  { (* read *)
+    inv STEP. ss.
+    esplits; [econs 2|].
+    - ss.
+    - econs; eauto.
+    - ss.
+  }
+  { (* fulfill *)
+    inv STEP. ss.
+    esplits; [econs 3|].
+    - ss.
+    - econs; eauto. ss.
+      inv WRITABLE. ss. econs; eauto. i. ss.
+    - ss.
+  }
+  { (* write failure *)
+    inv STEP. ss.
+  }
+  { (* fadd *)
+    inv STEP_READ. ss.
+    inv STEP_FULFILL. ss.
+    esplits; [econs 5|].
+    - ss.
+    - econs; eauto.
+    - econs; eauto. ss.
+      inv WRITABLE. ss. econs; eauto. i. ss.
+    - ss.
+  }
+  { (* isb *)
+    inv STEP. ss.
+    esplits; [econs 6|]; ss.
+  }
+  { (* dmb *)
+    inv STEP. ss.
+    esplits; [econs 7|]; ss.
+  }
+  { (* control *)
+    inv LC. ss.
+    esplits; [econs 8|]; ss.
+  }        
+Qed.
+
+
+Section RMWtoLLSC.
+  Hypothesis ARCH: arch = armv8.
+
+  Lemma rmw_to_llsc_sim_eu
+        tid tmp
+        stmts_src rmap_src lc_src mem_src
+        stmts_tgt rmap_tgt lc_tgt mem_tgt
+        (FRESH: List.Forall (fresh tmp) stmts_src)
+        (EXFREE: List.Forall exclusive_free stmts_src)
+        (STMTS: stmts_tgt = rmw_to_llsc_stmts tmp stmts_src)
+        (RMAP: sim_rmap tmp rmap_src rmap_tgt)
+        (LOCAL: sim_local lc_src lc_tgt)
+        (MEMORY: mem_src = mem_tgt):
+    @sim_eu tid
+            (ExecUnit.mk (State.mk stmts_src rmap_src) lc_src mem_src)
+            (ExecUnit.mk (State.mk stmts_tgt rmap_tgt) lc_tgt mem_tgt).
   Proof.
-    ii. econs.
-  Qed.
-  #[local] Hint Resolve sim_machine_monotone.
+    revert_until tmp.
+    pcofix CIH. i.
+    pfold. red. ss. subst. splits.
+    { (* terminal *)
+      i. red in TERMINAL_TGT. ss. des.
+      esplits; try refl. red. ss. split; cycle 1.
+      { inv LOCAL. congr. }
+      red in TERMINAL_TGT. red. ss.
+      destruct stmts_src; ss.
+      destruct s; ss. destruct i; ss.
+    }
 
-  Definition sim_machine := paco2 _sim_machine bot2.
-End SIM.
+    i. inv STEP_TGT. inv STEP. ss.
+    destruct stmts_src; try by inv STATE.
+    destruct eu2_tgt as [[stmts2_tgt rmap2_tgt] lc2_tgt mem2_tgt]. ss. subst.
+    exploit sim_local_step; try exact LOCAL0; eauto.
+    { destruct s; inv STATE; ss.
+      - destruct i; ss. inv H1.
+        inv EXFREE. inv H1. destruct ex0; ss.
+      - destruct i; ss. inv H1.
+        inv EXFREE. inv H1. destruct ex0; ss.
+    }
+    i. des.
+
+    destruct s; cycle 1.
+    { (* if *)
+      inv STATE.
+      eexists (ExecUnit.mk _ _ _). splits.
+      { econs 2; try refl. econs.
+        econs; try eapply STEP_SRC; ss.
+        econs; eauto.
+        admit. (* sem_expr *)
+      }
+      condtac; ss.
+      - right. eapply CIH; eauto.
+        + admit.
+        + admit.
+        + admit.
+      - right. eapply CIH; eauto.
+        + admit.
+        + admit.
+        + admit.
+    }
+
+    { (* while *)
+      inv STATE.
+      eexists (ExecUnit.mk _ _ _). splits.
+      { econs 2; try refl. econs.
+        econs; try eapply STEP_SRC; ss.
+        econs; eauto.
+      }
+      right. eapply CIH; eauto.
+      - admit.
+      - admit.
+      - admit.
+    }
+
+    admit.
+  Admitted.
+End RMWtoLLSC.
+
+
+Variant sim_sl (tmp: Id.t):
+  forall (sl_src sl_tgt: State.t (A:=View.t (A:=unit)) * Local.t (A:=unit)), Prop :=
+| sim_sl_intro
+    stmts_src rmap_src lc_src
+    stmts_tgt rmap_tgt lc_tgt
+    (STMTS: stmts_tgt = rmw_to_llsc_stmts tmp stmts_src)
+    (RMAP: sim_rmap tmp rmap_src rmap_tgt)
+    (LOCAL: lc_src = lc_tgt) (* TODO: fix *):
+  sim_sl tmp (State.mk stmts_src rmap_src, lc_src) (State.mk stmts_tgt rmap_tgt, lc_tgt)
+.
+
+Variant sim_machine (m_src m_tgt: Machine.t): Prop :=
+| sim_machine_intro
+    (TPOOL: forall tid, exists tmp,
+        option_rel (sim_sl tmp)
+                   (IdMap.find tid (Machine.tpool m_src))
+                   (IdMap.find tid (Machine.tpool m_tgt)))
+    (MEMORY: Machine.mem m_src = Machine.mem m_tgt)
+.
+
+
+Theorem rmw_to_llsc_sim
+        prog_src prog_tgt
+        (PROGRAM: rmw_to_llsc_program prog_src prog_tgt):
+  @sim sim_machine (Machine.init prog_src) (Machine.init prog_tgt).
+Proof.
+Admitted.
